sha/spec_hmac.v
@@ -57,9 +57,9 @@ Definition absCtxt (h:hmacabs): s256abs :=
   match h with HMACabs ctx _ _ _ _ => ctx end.
 
 Definition innerShaInit (k: list byte) (s:s256abs):Prop :=
-  update_abs (HMAC_SHA256.mkArgZ k HMAC_SHA256.Ipad) init_s256abs s.
+  update_abs (HMAC_SHA256.mkArgZ k Ipad) init_s256abs s.
 Definition outerShaInit (k: list byte) (s:s256abs):Prop :=
-  update_abs (HMAC_SHA256.mkArgZ k HMAC_SHA256.Opad) init_s256abs s.
+  update_abs (HMAC_SHA256.mkArgZ k Opad) init_s256abs s.
 
 Definition hmacInit (k:list Z) (h:hmacabs):Prop :=  
   let key := HMAC_SHA256.mkKey k in
@@ -106,7 +106,7 @@ Definition hmacSimple (k:list Z) (data:list Z) (dig:list Z) :=
 
 Lemma hmacSimple_sound k data dig: 
       hmacSimple k data dig ->
-      dig = HMAC_SHA256.HMAC data k.
+      dig = HMAC256 data k.
 Proof.
  unfold hmacSimple; intros [hInit [hUpd [HH1 [HH2 HH3]]]].
  unfold hmacInit in HH1. destruct HH1 as [iInit [oInit [HiInit [HoInit HINIT]]]]. subst.
@@ -119,7 +119,7 @@ Proof.
  inversion Hupd; clear Hupd. subst.
  unfold hmacFinalSimple in HH3. destruct HH3 as [oS [Upd FINISH]]. subst.
  inversion Upd; clear Upd. subst.
- unfold HMAC_SHA256.HMAC, HMAC_SHA256.OUTER, HMAC_SHA256.INNER.
+ unfold HMAC256, HMAC_SHA256.HMAC, HMAC_SHA256.OUTER, HMAC_SHA256.INNER.
  unfold sha_finish. unfold SHA256.Hash. rewrite functional_prog.SHA_256'_eq. f_equal.
  unfold HMAC_SHA256.innerArg, HMAC_SHA256.mkArgZ. rewrite H7. clear H7. 
  unfold HMAC_SHA256.outerArg, HMAC_SHA256.mkArgZ. rewrite H12. clear H12.
@@ -159,7 +159,7 @@ Qed.
 
 Lemma hmac_sound k data dig h: 
       hmac k data dig h ->
-      dig = HMAC_SHA256.HMAC data k.
+      dig = HMAC256 data k.
 Proof.
  intros.
  eapply hmacSimple_sound.
