sha/spec_hmacADT.v
@@ -51,9 +51,9 @@ Definition absCtxt (h:hmacabs): s256abs :=
   match h with HMACabs ctx _ _ => ctx end.
 
 Definition innerShaInit (k: list byte) (s:s256abs):Prop :=
-  update_abs (HMAC_SHA256.mkArgZ k HMAC_SHA256.Ipad) init_s256abs s.
+  update_abs (HMAC_SHA256.mkArgZ k Ipad) init_s256abs s.
 Definition outerShaInit (k: list byte) (s:s256abs):Prop :=
-  update_abs (HMAC_SHA256.mkArgZ k HMAC_SHA256.Opad) init_s256abs s.
+  update_abs (HMAC_SHA256.mkArgZ k Opad) init_s256abs s.
 
 Definition hmacInit (k:list Z) (h:hmacabs):Prop :=  
   let key := HMAC_SHA256.mkKey k in
@@ -159,7 +159,7 @@ Definition hmacSimple (k:list Z) (data:list Z) (dig:list Z) :=
 
 Lemma hmacSimple_sound k data dig: 
       hmacSimple k data dig ->
-      dig = HMAC_SHA256.HMAC data k.
+      dig = HMAC256 data k.
 Proof.
  unfold hmacSimple; intros [hInit [hUpd [HH1 [HH2 HH3]]]].
  unfold hmacInit in HH1. destruct HH1 as [iInit [oInit [HiInit [HoInit HINIT]]]]. subst.
@@ -172,7 +172,7 @@ Proof.
  inversion Hupd; clear Hupd. subst.
  unfold hmacFinalSimple in HH3. destruct HH3 as [oS [Upd FINISH]]. subst.
  inversion Upd; clear Upd. subst.
- unfold HMAC_SHA256.HMAC, HMAC_SHA256.OUTER, HMAC_SHA256.INNER.
+ unfold HMAC256, HMAC_SHA256.HMAC, HMAC_SHA256.OUTER, HMAC_SHA256.INNER.
  unfold sha_finish. unfold SHA256.Hash. 
  rewrite functional_prog.SHA_256'_eq. f_equal.
  unfold HMAC_SHA256.innerArg, HMAC_SHA256.mkArgZ. rewrite H7. clear H7. 
@@ -213,7 +213,7 @@ Qed.
 
 Lemma hmac_sound k data dig h: 
       hmac k data dig h ->
-      dig = HMAC_SHA256.HMAC data k.
+      dig = HMAC256 data k.
 Proof.
  intros.
  eapply hmacSimple_sound.
@@ -274,9 +274,9 @@ Definition initPre l (c:val) (k: val) h key : mpred:=
     Vint z => if Int.eq z Int.zero
               then hmacstate_PreInitNull key h c
               else FF
-  | Vptr b ofs => EX ll:Z,
+  | Vptr b ofs => EX ll:Z, EX CONT:_,
                   !!(has_lengthK ll key /\ l = Vint(Int.repr ll)) &&
-                  (data_at_ Tsh t_struct_hmac_ctx_st c) *
+                  (data_at Tsh t_struct_hmac_ctx_st CONT c) *
                         (data_block Tsh key (Vptr b ofs))
   | _ => FF
   end.
