sha/verif_hmacADT_simple.v
@@ -68,7 +68,8 @@ forward_call WITNESS.
      rewrite FR. clear FR Frame. 
   subst WITNESS. entailer. cancel. unfold initPre. 
    apply isptrD in Pkey'. destruct Pkey' as [kb [kofs HK]]. subst key'.
-   apply exp_right with (x:=kl). entailer. 
+   apply exp_right with (x:=kl). unfold data_at_. 
+   apply (exp_right (default_val t_struct_hmac_ctx_st)); entailer. 
 after_call.
 subst WITNESS. normalize. simpl. (* rewrite elim_globals_only'. normalize.
 simpl. *)
@@ -117,7 +118,7 @@ forward_call WITNESS.
       simpl in *. subst. unfold HMAC_SHA256.mkArgZ, HMAC_SHA256.mkArg in H10.
       assert (Zlength (map Byte.unsigned
         (map (fun p : byte * byte => Byte.xor (fst p) (snd p))
-           (combine (map Byte.repr (HMAC_SHA256.mkKey key)) (HMAC_SHA256.sixtyfour HMAC_SHA256.Ipad))))
+           (combine (map Byte.repr (HMAC_SHA256.mkKey key)) (HMAC_SHA256.sixtyfour Ipad))))
         = Zlength (SHA256.intlist_to_Zlist blocks ++ newfrag)).
         rewrite H10; reflexivity.
      clear H10.
